@WIP ftype recursion...

NS/TypesSubtype.v
@@ -26,8 +26,7 @@ Local Notation "a >= b" := (Bool.le b a) : bool_scope.
 
 (* Subtype relation *)
 Class Subtype (A: Set) := subtype: relation A.
-Class Subtype1 (F: Set -> Set) := subtype1: forall {A: Set}, relation A -> relation (F A).
-Global Instance unSubtype1 {F: Set -> Set} {C1: Subtype1 F} {A: Set} {C: Subtype A}: Subtype (F A) := subtype1 C.
+
 (* Definition wrapper prevents Coq from printing everything as a subtype relation
    while still printing explicitly defined subtype relations *)
 Definition ap_Subtype {A: Set} (S: Subtype A) (lhs rhs: A) := S lhs rhs.
@@ -56,152 +55,113 @@ Notation "'(I)'" := Intersection.
 Notation "lhs 'I' rhs '=' a" := (Intersection lhs rhs a) (at level 60, rhs at next level, no associativity).
 
 Class EqvType (A: Set) := eqv_type: relation A.
-Class EqvType1 (F: Set -> Set) := eqv_type1: forall {A: Set}, relation A -> relation (F A).
-Global Instance unEqvType1 {F: Set -> Set} {C1: EqvType1 F} {A: Set} {C: EqvType A}: EqvType (F A) := eqv_type1 C.
 Definition ap_EqvType {A: Set} (S: EqvType A) (lhs rhs: A) := S lhs rhs.
 Notation "'[' eqv_type ']' lhs '==' rhs" := (ap_EqvType eqv_type lhs rhs) (at level 60, lhs at next level, rhs at next level, no associativity).
 Notation "lhs '==' rhs" := (eqv_type lhs rhs) (at level 60, rhs at next level, no associativity).
 
 Class IsValidType (A: Set) := is_valid_type: A -> Prop.
-Class IsValidType1 (F: Set -> Set) := is_valid_type1: forall {A: Set}, (A -> Prop) -> (F A -> Prop).
-Global Instance unIsValidType1 {F: Set -> Set} {C1: IsValidType1 F} {A: Set} {C: IsValidType A}: IsValidType (F A) := is_valid_type1 C.
-Definition unIsValidType1' {F: Set -> Set} {A: Set} `{C1: IsValidType1 F} `{C: IsValidType A}: forall a, is_valid_type1 C a -> is_valid_type a.
-  intros; unfold is_valid_type, unIsValidType1; exact H. Defined.
 Definition IsValidType_always {A: Set}: IsValidType A := fun _ => True.
 
 (* Subtype properties *)
 Unset Implicit Arguments.
 Class Top (A: Set): Set := top: A.
-Class Top1 (F: Set -> Set) := top1: forall {A: Set}, Top A -> F A.
-Global Instance unTop1 {F: Set -> Set} {C1: Top1 F} {A: Set} {C: Top A}: Top (F A) := top1 C.
 Class Bottom (A: Set): Set := bottom: A.
-Class Bottom1 (F: Set -> Set) := bottom1: forall {A: Set}, Bottom A -> F A.
-Global Instance unBottom1 {F: Set -> Set} {C1: Bottom1 F} {A: Set} {C: Bottom A}: Bottom (F A) := bottom1 C.
-Class SubtypeTop (A: Set) `{_Subtype: Subtype A} `{_Top: Top A}: Prop := subtype_top: forall (a: A), a <: top.
-Class SubtypeTop1 (F: Set -> Set) `{_Subtype1: Subtype1 F} `{_Top1: Top1 F}: Prop := subtype_top1: forall {A: Set} `{_Subtype: Subtype A} `{_Top: Top A}, SubtypeTop A -> SubtypeTop (F A).
-Global Instance unSubtypeTop1 {F: Set -> Set} `{C1: SubtypeTop1 F} {A: Set} `{C: SubtypeTop A}: SubtypeTop (F A) := subtype_top1 C.
-Class SubtypeBottom (A: Set) `{_Subtype: Subtype A} `{_Bottom: Bottom A}: Prop := subtype_bottom: forall (a: A), bottom <: a.
-Class SubtypeBottom1 (F: Set -> Set) `{_Subtype1: Subtype1 F} `{_Bottom1: Bottom1 F}: Prop := subtype_bottom1: forall {A: Set} {_Subtype: Subtype A} {_Bottom: Bottom A}, SubtypeBottom A -> SubtypeBottom (F A).
-Global Instance unSubtypeBottom1 {F: Set -> Set} `{C1: SubtypeBottom1 F} {A: Set} `{C: SubtypeBottom A}: SubtypeBottom (F A) := subtype_bottom1 C.
-Class SubtypeRefl (A: Set) `{_Subtype: Subtype A} `{_IsValidType: IsValidType A}: Prop := subtype_refl: forall (a: A), is_valid_type a -> a <: a.
-Class SubtypeRefl1 (F: Set -> Set) `{_Subtype1: Subtype1 F} `{_IsValidType1: IsValidType1 F}: Prop := subtype_refl1: forall {A: Set} `{_Subtype: Subtype A} `{_IsValidType: IsValidType A}, SubtypeRefl A -> SubtypeRefl (F A).
-Global Instance unSubtypeRefl1 {F: Set -> Set} `{C1: SubtypeRefl1 F} {A: Set} `{C: SubtypeRefl A}: SubtypeRefl (F A) := subtype_refl1 C.
-Class SubtypeAntisym (A: Set) `{_Subtype: Subtype A} `{_EqvType: EqvType A}: Prop := subtype_antisym: forall (a b: A), a <: b -> b <: a -> a == b.
-Class SubtypeAntisym1 (F: Set -> Set) `{_Subtype1: Subtype1 F} `{_EqvType1: EqvType1 F}: Prop := subtype_antisym1: forall {A: Set} `{_Subtype: Subtype A} `{_EqvType: EqvType A}, SubtypeAntisym A -> SubtypeAntisym (F A).
-Global Instance unSubtypeAntisym1 {F: Set -> Set} `{C1: SubtypeAntisym1 F} {A: Set} `{C: SubtypeAntisym A}: SubtypeAntisym (F A) := subtype_antisym1 C.
-Class SubtypeTrans (A: Set) `{_Subtype: Subtype A}: Prop := subtype_trans: forall (a b c: A), a <: b -> b <: c -> a <: c.
-Class SubtypeTrans1 (F: Set -> Set) `{_Subtype1: Subtype1 F}: Prop := subtype_trans1: forall {A: Set} `{_Subtype: Subtype A}, SubtypeTrans A -> SubtypeTrans (F A).
-Global Instance unSubtypeTrans1 {F: Set -> Set} `{C1: SubtypeTrans1 F} {A: Set} `{C: SubtypeTrans A}: SubtypeTrans (F A) := subtype_trans1 C.
-Class SubtypeValid (A: Set) `{_Subtype: Subtype A} `{_IsValidType: IsValidType A} `{_EqvType: EqvType A}: Prop := subtype_valid: SubtypeRefl A /\ SubtypeAntisym A /\ SubtypeTrans A.
-Class SubtypeValid0 (A: Set) `{_Subtype: Subtype A} `{_IsValidType: IsValidType A} `{_EqvType: EqvType A} `{_Top: Top A} `{_Bottom: Bottom A}: Prop := subtype_valid0: SubtypeTop A /\ SubtypeBottom A /\ SubtypeValid A.
+Class SubtypeTop {A: Set} `(S: Subtype A) `{_Top: Top A}: Prop := subtype_top: forall (a: A), a <: top.
+Class SubtypeBottom {A: Set} `(S: Subtype A) `{_Bottom: Bottom A}: Prop := subtype_bottom: forall (a: A), bottom <: a.
+Class SubtypeRefl {A: Set} `(S: Subtype A) `{V: IsValidType A}: Prop := subtype_refl: forall (a: A), is_valid_type a -> a <: a.
+Class SubtypeAntisym {A: Set} `(S: Subtype A) `{E: EqvType A}: Prop := subtype_antisym: forall (a b: A), a <: b -> b <: a -> a == b.
+Class SubtypeTrans {A: Set} `(S: Subtype A): Prop := subtype_trans: forall (a b c: A), a <: b -> b <: c -> a <: c.
+Class SubtypeValid {A: Set} `(S: Subtype A) `{V: IsValidType A} `{E: EqvType A}: Prop := subtype_valid: SubtypeRefl S /\ SubtypeAntisym S /\ SubtypeTrans S.
+Class SubtypeValid0 {A: Set} `(S: Subtype A) `{V: IsValidType A} `{E: EqvType A} `{_Top: Top A} `{_Bottom: Bottom A}: Prop := subtype_valid0: SubtypeTop S /\ SubtypeBottom S /\ SubtypeValid S.
 (* TODO: Some of these = may need to be == *)
-Class UnionTop (A: Set) `{_Subtype: Subtype A} `{_Top: Top A}: Prop := union_top: forall (a: A), top U a = top.
-Class UnionBottom (A: Set) `{_Subtype: Subtype A} `{_Bottom: Bottom A}: Prop := union_bottom: forall (a: A), bottom U a = a.
-Class IntersectTop (A: Set) `{_Subtype: Subtype A} `{_Top: Top A}: Prop := intersect_top: forall (a: A), top I a = a.
-Class IntersectBottom (A: Set) `{_Subtype: Subtype A} `{_Bottom: Bottom A}: Prop := intersect_bottom: forall (a: A), bottom I a = bottom.
-Class UnionRefl (A: Set) `{_Subtype: Subtype A} `{_IsValidType: IsValidType A}: Prop := union_refl: forall (a: A), is_valid_type a -> a U a = a.
-Class IntersectRefl (A: Set) `{_Subtype: Subtype A} `{_IsValidType: IsValidType A}: Prop := intersect_refl: forall (a: A), is_valid_type a -> a I a = a.
-Class UnionComm (A: Set) `{_Subtype: Subtype A}: Prop := union_comm: forall (a b ab: A), a U b = ab <-> b U a = ab.
-Class IntersectComm (A: Set) `{_Subtype: Subtype A}: Prop := intersect_comm: forall (a b ab: A), a I b = ab <-> b I a = ab.
-Class UnionAssoc (A: Set) `{_Subtype: Subtype A}: Prop := union_assoc: forall (a b c ab bc abc: A), a U b = ab -> b U c = bc -> ab U c = abc <-> a U bc = abc.
-Class IntersectAssoc (A: Set) `{_Subtype: Subtype A}: Prop := intersect_assoc: forall (a b c ab bc abc: A), a I b = ab -> b I c = bc -> ab I c = abc <-> a I bc = abc.
-Class UnionAbsorb (A: Set) `{_Subtype: Subtype A}: Prop := union_absorb: forall (a b ab: A), a <: b -> a U b = ab <-> a = ab.
-Class IntersectAbsorb (A: Set) `{_Subtype: Subtype A}: Prop := intersect_absorb: forall (a b ab: A), a <: b -> a I b = ab <-> b = ab.
-Class UnionIntersectValid (A: Set) `{_Subtype: Subtype A} `{_IsValidType: IsValidType A}: Prop := union_intersect_valid: UnionRefl A /\ IntersectRefl A /\ UnionComm A /\ IntersectComm A /\ UnionAssoc A /\ IntersectAssoc A /\ UnionAbsorb A /\ IntersectAbsorb A.
-Class UnionIntersectValid0 (A: Set) `{_Subtype: Subtype A} `{_IsValidType: IsValidType A} `{_Top: Top A} `{_Bottom: Bottom A}: Prop := union_intersect_valid0: UnionBottom A /\ UnionTop A /\ IntersectBottom A /\ IntersectTop A /\ UnionIntersectValid A.
-Class UnionSubtypeLattice0 (A: Set) `{_Subtype: Subtype A}: Prop := union_subtype_lattice0: forall (a b ab c: A), a <: c -> b <: c -> a U b = ab -> ab <: c.
-Class IntersectSubtypeLattice0 (A: Set) `{_Subtype: Subtype A}: Prop := intersect_subtype_lattice0: forall (a b ab c: A), c <: a -> c <: b -> a I b = ab -> c <: ab.
-Class UnionSubtypeLattice1 (A: Set) `{_Subtype: Subtype A}: Prop := union_subtype_lattice1: forall (a b c d ab cd: A), a <: c -> b <: d -> a U b = ab -> c U d = cd -> ab <: cd.
-Class IntersectSubtypeLattice1 (A: Set) `{_Subtype: Subtype A}: Prop := intersect_subtype_lattice1: forall (a b c d ab cd: A), a <: c -> b <: d -> a I b = ab -> c I d = cd -> ab <: cd.
-Class UnionSubtypeLattice2 (A: Set) `{_Subtype: Subtype A}: Prop := union_subtype_lattice2: forall (a b ab: A), a U b = ab -> a <: ab /\ b <: ab.
-Class IntersectSubtypeLattice2 (A: Set) `{_Subtype: Subtype A}: Prop := intersect_subtype_lattice2: forall (a b ab: A), a I b = ab -> ab <: a /\ ab <: b.
-Class UnionIntersectSubtypeLattice (A: Set) `{_Subtype: Subtype A} `{_Top: Top A} `{_Bottom: Bottom A}: Prop := union_intersectSubtype_lattice: UnionSubtypeLattice0 A /\ UnionSubtypeLattice1 A /\ UnionSubtypeLattice2 A /\ IntersectSubtypeLattice0 A /\ IntersectSubtypeLattice1 A /\ IntersectSubtypeLattice2 A.
-Class SubtypeUnionIntersectValid (A: Set) `{_Subtype: Subtype A} `{_IsValidType: IsValidType A} `{_EqvType: EqvType A} `{_Top: Top A} `{_Bottom: Bottom A}: Prop := subtype_union_intersect_valid: SubtypeValid A /\ UnionIntersectValid A /\ UnionIntersectSubtypeLattice A.
+Class UnionTop {A: Set} `(S: Subtype A) `{_Top: Top A}: Prop := union_top: forall (a: A), top U a = top.
+Class UnionBottom {A: Set} `(S: Subtype A) `{_Bottom: Bottom A}: Prop := union_bottom: forall (a: A), bottom U a = a.
+Class IntersectTop {A: Set} `(S: Subtype A) `{_Top: Top A}: Prop := intersect_top: forall (a: A), top I a = a.
+Class IntersectBottom {A: Set} `(S: Subtype A) `{_Bottom: Bottom A}: Prop := intersect_bottom: forall (a: A), bottom I a = bottom.
+Class UnionRefl {A: Set} `(S: Subtype A) `{V: IsValidType A}: Prop := union_refl: forall (a: A), is_valid_type a -> a U a = a.
+Class IntersectRefl {A: Set} `(S: Subtype A) `{V: IsValidType A}: Prop := intersect_refl: forall (a: A), is_valid_type a -> a I a = a.
+Class UnionComm {A: Set} `(S: Subtype A): Prop := union_comm: forall (a b ab: A), a U b = ab <-> b U a = ab.
+Class IntersectComm {A: Set} `(S: Subtype A): Prop := intersect_comm: forall (a b ab: A), a I b = ab <-> b I a = ab.
+Class UnionAssoc {A: Set} `(S: Subtype A): Prop := union_assoc: forall (a b c ab bc abc: A), a U b = ab -> b U c = bc -> ab U c = abc <-> a U bc = abc.
+Class IntersectAssoc {A: Set} `(S: Subtype A): Prop := intersect_assoc: forall (a b c ab bc abc: A), a I b = ab -> b I c = bc -> ab I c = abc <-> a I bc = abc.
+Class UnionAbsorb {A: Set} `(S: Subtype A): Prop := union_absorb: forall (a b ab: A), a <: b -> a U b = ab <-> a = ab.
+Class IntersectAbsorb {A: Set} `(S: Subtype A): Prop := intersect_absorb: forall (a b ab: A), a <: b -> a I b = ab <-> b = ab.
+Class UnionIntersectValid {A: Set} `(S: Subtype A) `{V: IsValidType A}: Prop := union_intersect_valid: UnionRefl S /\ IntersectRefl S /\ UnionComm S /\ IntersectComm S /\ UnionAssoc S /\ IntersectAssoc S /\ UnionAbsorb S /\ IntersectAbsorb S.
+Class UnionIntersectValid0 {A: Set} `(S: Subtype A) `{V: IsValidType A} `{_Top: Top A} `{_Bottom: Bottom A}: Prop := union_intersect_valid0: UnionBottom S /\ UnionTop S /\ IntersectBottom S /\ IntersectTop S /\ UnionIntersectValid S.
+Class UnionSubtypeLattice0 {A: Set} `(S: Subtype A): Prop := union_subtype_lattice0: forall (a b ab c: A), a <: c -> b <: c -> a U b = ab -> ab <: c.
+Class IntersectSubtypeLattice0 {A: Set} `(S: Subtype A): Prop := intersect_subtype_lattice0: forall (a b ab c: A), c <: a -> c <: b -> a I b = ab -> c <: ab.
+Class UnionSubtypeLattice1 {A: Set} `(S: Subtype A): Prop := union_subtype_lattice1: forall (a b c d ab cd: A), a <: c -> b <: d -> a U b = ab -> c U d = cd -> ab <: cd.
+Class IntersectSubtypeLattice1 {A: Set} `(S: Subtype A): Prop := intersect_subtype_lattice1: forall (a b c d ab cd: A), a <: c -> b <: d -> a I b = ab -> c I d = cd -> ab <: cd.
+Class UnionSubtypeLattice2 {A: Set} `(S: Subtype A): Prop := union_subtype_lattice2: forall (a b ab: A), a U b = ab -> a <: ab /\ b <: ab.
+Class IntersectSubtypeLattice2 {A: Set} `(S: Subtype A): Prop := intersect_subtype_lattice2: forall (a b ab: A), a I b = ab -> ab <: a /\ ab <: b.
+Class UnionIntersectSubtypeLattice {A: Set} `(S: Subtype A) `{_Top: Top A} `{_Bottom: Bottom A}: Prop := union_intersectSubtype_lattice: UnionSubtypeLattice0 S /\ UnionSubtypeLattice1 S /\ UnionSubtypeLattice2 S /\ IntersectSubtypeLattice0 S /\ IntersectSubtypeLattice1 S /\ IntersectSubtypeLattice2 S.
+Class SubtypeUnionIntersectValid {A: Set} `(S: Subtype A) `{V: IsValidType A} `{E: EqvType A} `{_Top: Top A} `{_Bottom: Bottom A}: Prop := subtype_union_intersect_valid: SubtypeValid S /\ UnionIntersectValid S /\ UnionIntersectSubtypeLattice S.
 Set Implicit Arguments.
 
 (* Subtype relation implementations *)
 Inductive S_option {A: Set} (S: Subtype A): Subtype (option A) :=
 | S_None            : forall (lhs: option A), [S_option S] lhs <: None
 | S_Some            : forall (lhs rhs: A), [S] lhs <: rhs -> [S_option S] Some lhs <: Some rhs
-. Global Instance SOf_option {A: Set} {S: Subtype A}: Subtype (option A) := S_option S.
-Global Instance S1Of_option: Subtype1 option := @S_option.
+. Global Existing Instance S_option.
 Inductive E_option {A: Set} (E: EqvType A) : EqvType (option A) :=
 | E_None            : forall (lhs: option A), [E_option E] lhs == None
 | E_Some            : forall (lhs rhs: A), [E] lhs == rhs -> [E_option E] (Some lhs) == (Some rhs)
-. Global Instance EOf_option {A: Set} {E: EqvType A}: EqvType (option A) := E_option E.
-Global Instance E1Of_option: EqvType1 option := @E_option.
+. Global Existing Instance E_option.
 Inductive S_Zip {A: Set} (S: Subtype A): Subtype (list A) :=
 | S_Zip_nil          : forall (lhs: list A), [S_Zip S] lhs <: nil
 | S_Zip_cons         : forall (l r: A) (ls rs: list A),
     [S] l <: r -> [S_Zip S] ls <: rs -> [S_Zip S] (l :: ls) <: (r :: rs)
-(* no global instance because there is S_Intersect *)
-. Definition SOf_Zip {A: Set} {S: Subtype A}: Subtype (list A) := S_Zip S.
-Definition S1Of_Zip: Subtype1 list := @S_Zip.
+.
 Inductive E_Zip {A: Set} (E: EqvType A) : EqvType (list A) :=
 | E_Zip_nil          : [E_Zip E] nil == nil
 | E_Zip_cons         : forall (l r: A) (ls rs: list A),
     [E] l == r -> [E_Zip E] ls == rs -> [E_Zip E] (l :: ls) == (r :: rs)
-. Global Instance EOf_Zip {A: Set} {E: EqvType A}: EqvType (list A) := E_Zip E.
-Global Instance E1Of_Zip: EqvType1 list := @E_Zip.
-(* no global instance because there is S_Zip and S_Intersect *)
-Definition S_JsrZip {A: Set} (S: Subtype A): Subtype (js_record A) := JsRecord1Rel S.
-Definition SOf_JsrZip {A: Set} {S: Subtype A}: Subtype (js_record A) := JsRecord1Rel S.
-Definition S1Of_JsrZip: Subtype1 js_record := @S_JsrZip.
-Global Instance EOf_JsrZip {A: Set} {E: EqvType A}: EqvType (js_record A) := JsRecordRel E.
-Global Instance E1Of_JsrZip: EqvType1 js_record := @EOf_JsrZip.
+. Global Existing Instance E_Zip.
+Global Instance S_JsrZip {A: Set} (S: Subtype A): Subtype (js_record A) := JsRecord1Rel S.
+Global Instance E_JsrZip {A: Set} (E: EqvType A): EqvType (js_record A) := JsRecordRel E.
 Inductive S_Intersect {A: Set} (S: Subtype A): Subtype (list A) :=
 | S_Intersect_nil    : forall (lhs: list A), [S_Intersect S] lhs <: nil
 | S_Intersect_cons   : forall (l r: A) (ls rs: list A),
     [S] l <: r -> [S_Intersect S] ls <: rs -> [S_Intersect S] (l :: ls) <: (r :: rs)
 | S_Intersect_cons_l : forall (l: A) (ls rs: list A),
                  [S_Intersect S] ls <: rs -> [S_Intersect S] (l :: ls) <: rs
-(* no global instance because there is S_Zip *)
-. Definition SOf_Intersect {A: Set} {S: Subtype A}: Subtype (list A) := S_Intersect S.
-Definition S1Of_Intersect: Subtype1 list := @S_Intersect.
+.
 Inductive S_variance: Subtype variance :=
 | S_Bivariant        : forall (lhs: variance), [S_variance] lhs <: Bivariant
 | S_Covariant        : [S_variance] Covariant <: Covariant
 | S_Contravariant    : [S_variance] Contravariant <: Contravariant
 | S_Invariant        : forall (rhs: variance), [S_variance] Invariant <: rhs
-. Global Instance SOf_variance: Subtype variance := S_variance.
-Global Instance EOf_variance: EqvType variance := eq.
+. Global Existing Instance S_variance.
+Global Instance E_variance: EqvType variance := eq.
 Inductive S_otype {A: Set} (S: Subtype A): Subtype (otype A) :=
 | S_OType            : forall (ol or: bool) (lhs rhs: A), ol <= or -> [S] lhs <: rhs -> [S_otype S] Ot ol lhs <: Ot or rhs
-. Global Instance SOf_otype {A: Set} {S: Subtype A}: Subtype (otype A) := S_otype S.
-Global Instance S1Of_otype: Subtype1 otype := @S_otype.
+. Global Existing Instance S_otype.
 Inductive E_otype {A: Set} (E: EqvType A): EqvType (otype A) :=
 | E_OType            : forall (o: bool) (lhs rhs: A), [E] lhs == rhs -> [E_otype E] Ot o lhs == Ot o rhs
-. Global Instance EOf_otype {A: Set} {E: EqvType A}: EqvType (otype A) := E_otype E.
-Global Instance E1Of_otype: EqvType1 otype := @E_otype.
+. Global Existing Instance E_otype.
 Inductive S_vtype {A: Set} (S: Subtype A): Subtype (vtype A) :=
 | S_Void             : [S_vtype S] @VVoid A <: VVoid
 | S_NotVoid          : forall (lhs rhs: A), [S] lhs <: rhs -> [S_vtype S] Vt lhs <: Vt rhs
-. Global Instance SOf_vtype {A: Set} {S: Subtype A}: Subtype (vtype A) := S_vtype S.
-Global Instance S1Of_vtype: Subtype1 vtype := @S_vtype.
+. Global Existing Instance S_vtype.
 Inductive E_vtype {A: Set} (E: EqvType A): EqvType (vtype A) :=
 | E_Void             : [E_vtype E] @VVoid A == VVoid
 | E_NotVoid          : forall (lhs rhs: A), [E] lhs == rhs -> [E_vtype E] Vt lhs == Vt rhs
-. Global Instance EOf_vtype {A: Set} {E: EqvType A}: EqvType (vtype A) := E_vtype E.
-Global Instance E1Of_vtype: EqvType1 vtype := @E_vtype.
+. Global Existing Instance E_vtype.
 Inductive S_tparam {A: Set} (S: Subtype A): Subtype (tparam A) :=
 | S_TParam           : forall (vl vr: variance) (name: string) (supl supr: list A),
     [S_variance] vl <: vr -> [S_Intersect S] supl <: supr ->
     [S_tparam S] TParam vl name supl <: TParam vr name supr
-. Global Instance SOf_tparam {A: Set} {S: Subtype A}: Subtype (tparam A) := S_tparam S.
-Global Instance S1Of_tparam: Subtype1 tparam := @S_tparam.
+. Global Existing Instance S_tparam.
 Inductive E_tparam {A: Set} (E: EqvType A): EqvType (tparam A) :=
 | E_TParam           : forall (v: variance) (name: string) (supl supr: list A),
     [E_Zip E] supl == supr -> [E_tparam E] TParam v name supl == TParam v name supr
-. Global Instance EOf_tparam {A: Set} {E: EqvType A}: EqvType (tparam A) := E_tparam E.
-Global Instance E1Of_tparam: EqvType1 tparam := @E_tparam.
+. Global Existing Instance E_tparam.
 Inductive S_itype {A: Set} (S: Subtype A): Subtype (itype A) :=
 | S_Ident            : forall (name: string) (tal tar: list A), [S_Zip S] tal <: tar -> [S_itype S] It name tal <: It name tar
-. Global Instance SOf_itype {A: Set} {S: Subtype A}: Subtype (itype A) := S_itype S.
-Global Instance S1Of_itype: Subtype1 itype := @S_itype.
+. Global Existing Instance S_itype.
 Inductive E_itype {A: Set} (E: EqvType A): EqvType (itype A) :=
 | E_Ident            : forall (name: string) (tal tar: list A), [E_Zip E] tal == tar -> [E_itype E] It name tal == It name tar
-. Global Instance EOf_itype {A: Set} {E: EqvType A}: EqvType (itype A) := E_itype E.
-Global Instance E1Of_itype: EqvType1 itype := @E_itype.
+. Global Existing Instance E_itype.
 Inductive S_stype {A: Set} (S: Subtype A): Subtype (stype A) :=
 | S_Fn               : forall (tpl tpr: list (tparam A)) (thispl thispr: A)
                          (pl pr: list (otype A)) (rl rr: A) (retl retr: (vtype A)),
@@ -210,8 +170,7 @@ Inductive S_stype {A: Set} (S: Subtype A): Subtype (stype A) :=
 | S_Array            : forall (el er: A),                     [S]                     el <: er  -> [S_stype S] SArray el   <: SArray er
 | S_Tuple            : forall (esl esr: list (otype A)),      [S_Zip (S_otype S)]    esl <: esr -> [S_stype S] STuple esl  <: STuple esr
 | S_Object           : forall (fsl fsr: js_record (otype A)), [S_JsrZip (S_otype S)] fsl <: fsr -> [S_stype S] SObject fsl <: SObject fsr
-. Global Instance SOf_stype {A: Set} {S: Subtype A}: Subtype (stype A) := S_stype S.
-Global Instance S1Of_stype: Subtype1 stype := @S_stype.
+. Global Existing Instance S_stype.
 Inductive E_stype {A: Set} (E: EqvType A): EqvType (stype A) :=
 | E_Fn               : forall (tpl tpr: list (tparam A)) (thispl thispr: A)
                          (pl pr: list (otype A)) (rl rr: A) (retl retr: (vtype A)),
@@ -220,8 +179,7 @@ Inductive E_stype {A: Set} (E: EqvType A): EqvType (stype A) :=
 | E_Array            : forall (el er: A),                     [E]                     el == er  -> [E_stype E] SArray el   == SArray er
 | E_Tuple            : forall (esl esr: list (otype A)),      [E_Zip (E_otype E)]    esl == esr -> [E_stype E] STuple esl  == STuple esr
 | E_Object           : forall (fsl fsr: js_record (otype A)), [JsRecordRel (E_otype E)] fsl == fsr -> [E_stype E] SObject fsl == SObject fsr
-. Global Instance EOf_stype {A: Set} {E: EqvType A}: EqvType (stype A) := E_stype E.
-Global Instance E1Of_stype: EqvType1 stype := @E_stype.
+. Global Existing Instance E_stype.
 Inductive S_ftype: Subtype ftype :=
 | S_Any              : forall (lhs: ftype), [S_ftype] lhs <: FAny
 | S_Never            : forall (rhs: ftype), [S_ftype] FNEVER <: rhs
@@ -233,7 +191,7 @@ Inductive S_ftype: Subtype ftype :=
 | S_Nom              : forall (nl nr: bool) (idl idr: iftype) (idsl idsr: list iftype) (sl sr: option sftype),
     nl <= nr -> [S_Intersect (S_itype S_ftype)] (idl :: idsl) <: (idr :: idsr) -> [S_option (S_stype S_ftype)] sl <: sr ->
     [S_ftype] FNominal nl idl idsl sl <: FNominal nr idr idsr sr
-. Global Instance SOf_ftype: Subtype ftype := S_ftype.
+. Global Existing Instance S_ftype.
 Inductive E_ftype: EqvType ftype :=
 | E_Any              : [E_ftype] FAny == FAny
 | E_NeverNull        : forall (n: bool), [E_ftype] FNever n == FNever n
@@ -242,78 +200,91 @@ Inductive E_ftype: EqvType ftype :=
 | E_Nom              : forall (n: bool) (idl idr: iftype) (idsl idsr: list iftype) (sl sr: option sftype),
     [E_Zip (E_itype E_ftype)] (idl :: idsl) == (idr :: idsr) -> [E_option (E_stype E_ftype)] sl == sr ->
     [E_ftype] FNominal n idl idsl sl == FNominal n idr idsr sr
-. Global Instance EOf_ftype: EqvType ftype := E_ftype.
+. Global Existing Instance E_ftype.
 
-(* An axiom needed for induction because of complex recursion *)
-Axiom S_ftype_ind':
-  forall (P: Subtype ftype)
-    (fS_Any: forall lhs : ftype, P lhs FAny)
-    (fS_Never: forall rhs : ftype, P FNEVER rhs)
-    (fS_Null: forall rhs : ftype, IsNullable rhs -> P FNULL rhs)
-    (fS_Struct: forall (nl nr : bool) (sl sr : sftype),
-      nl <= nr ->
-      [S_stype P] sl <: sr ->
-      P (FStructural nl sl) (FStructural nr sr))
-    (fS_NomStruct: forall (nl nr : bool) (idl : iftype) (idsl : list iftype) (sl sr : sftype),
-      nl <= nr ->
-      [S_stype P] sl <: sr ->
-      P (FNominal nl idl idsl (Some sl)) (FStructural nr sr))
-    (fS_Nom: forall (nl nr : bool) (idl idr idu : iftype) (idsl idsr idsu : list iftype)
-        (sl sr su : option sftype),
-      nl <= nr ->
-      [S_Intersect (S_itype P)] (idl :: idsl) <: (idr :: idsr) ->
-      [S_option (S_stype P)] sl <: sr ->
-      P (FNominal nl idl idsl sl) (FNominal nr idr idsr sr))
-    (lhs rhs: ftype), S_ftype lhs rhs -> P lhs rhs.
-Axiom E_ftype_ind':
-  forall (P: EqvType ftype)
-    (fE_Any: P FAny FAny)
-    (fE_NeverNull: forall (n : bool), P (FNever n) (FNever n))
-    (fE_Struct: forall (n : bool) (sl sr : sftype),
-      [E_stype P] sl == sr -> P (FStructural n sl) (FStructural n sr))
-    (fE_Nom: forall (n : bool) (idl idr idu : iftype) (idsl idsr idsu : list iftype) (sl sr su : option sftype),
-      [E_Zip (E_itype P)] (idl :: idsl) == (idr :: idsr) ->
-      [E_option (E_stype P)] sl == sr ->
-      P (FNominal n idl idsl sl) (FNominal n idr idsr sr))
-    (lhs rhs: ftype), E_ftype lhs rhs -> P lhs rhs.
+Global Instance Top_option {A: Set} `{_Top: Top A}: Top (option A) := None.
+Global Instance Bottom_option {A: Set} `{_Bottom: Bottom A}: Bottom (option A) := Some bottom.
+Global Instance Top_variance: Top variance := Bivariant.
+Global Instance Bottom_variance: Bottom variance := Invariant.
+Global Instance Top_otype {A: Set} `{_Top: Top A}: Top (otype A) := Ot true _Top.
+Global Instance Bottom_otype {A: Set} `{_Bottom: Bottom A}: Bottom (otype A) := Ot false _Bottom.
+Global Instance Top_ftype: Top ftype := FAny.
+Global Instance Bottom_ftype: Bottom ftype := FNEVER.
+
+Global Instance IsValidType_option {A: Set} `{V: IsValidType A}: IsValidType (option A) := Option_Forall V.
+Global Instance IsValidType_list {A: Set} `{V: IsValidType A}: IsValidType (list A) := List.Forall V.
+Global Instance IsValidType_js_record {A: Set} `{V: IsValidType A}: IsValidType (js_record A) := JsRecordNoDupForall V.
+Global Instance IsValidType_variance: IsValidType variance := IsValidType_always.
+Global Instance IsValidType_otype {A: Set} `{V: IsValidType A}: IsValidType (otype A) := OType_Forall V.
+Global Instance IsValidType_vtype {A: Set} `{V: IsValidType A}: IsValidType (vtype A) := VType_Forall V.
+Global Instance IsValidType_tparam {A: Set} `{V: IsValidType A}: IsValidType (tparam A) := TParam_Forall V.
+Global Instance IsValidType_itype {A: Set} `{V: IsValidType A}: IsValidType (itype A) := IType_Forall V.
+Global Instance IsValidType_stype {A: Set} `{V: IsValidType A}: IsValidType (stype A) := SType_Forall' V.
+Inductive IsValidType_ftype: IsValidType ftype :=
+| FAny: IsValidType_ftype FAny
+| FNever: forall x, IsValidType_ftype (FNever x)
+| FStructural: forall x structure, @IsValidType_stype ftype IsValidType_ftype structure -> IsValidType_ftype (FStructural x structure)
+| FNominal: forall x id sids structure, @IsValidType_itype ftype IsValidType_ftype id -> @IsValidType_list iftype (@IsValidType_itype ftype IsValidType_ftype) sids -> @IsValidType_option sftype (@IsValidType_stype ftype IsValidType_ftype) structure -> IsValidType_ftype (FNominal x id sids structure)
+. Global Existing Instance IsValidType_ftype.
+
+(* Axiom because I have no idea how to handle the complex recursion or if its even possible *)
+Axiom S_ftype_ind0:
+  forall (P: forall {A: Set} {V: IsValidType A}, Subtype A -> Prop)
+    (f_option: forall {A: Set} {S: Subtype A} {V: IsValidType A}, P S -> P (S_option S))
+    (f_Zip: forall {A: Set} {S: Subtype A} {V: IsValidType A}, P S -> P (S_Zip S))
+    (f_Intersect: forall {A: Set} {S: Subtype A} {V: IsValidType A}, P S -> P (S_Intersect S))
+    (f_vtype: forall {A: Set} {S: Subtype A} {V: IsValidType A}, P S -> P (S_vtype S))
+    (f_otype: forall {A: Set} {S: Subtype A} {V: IsValidType A}, P S -> P (S_otype S))
+    (f_tparam: forall {A: Set} {S: Subtype A} {V: IsValidType A}, P S -> P (S_tparam S))
+    (f_itype: forall {A: Set} {S: Subtype A} {V: IsValidType A}, P S -> P (S_itype S))
+    (f_stype: forall {A: Set} {S: Subtype A} {V: IsValidType A}, P S -> P (S_stype S))
+    (f_variance: P S_variance),
+    (P S_ftype -> P S_ftype) -> P S_ftype.
+Axiom S_ftype_ind1:
+  forall (P: forall {A: Set} {V: IsValidType A} {E: EqvType A}, Subtype A -> Prop)
+    (f_option: forall {A: Set} {S: Subtype A} {V: IsValidType A} {E: EqvType A}, P S -> P (S_option S))
+    (f_Zip: forall {A: Set} {S: Subtype A} {V: IsValidType A} {E: EqvType A}, P S -> P (S_Zip S))
+    (f_Intersect: forall {A: Set} {S: Subtype A} {V: IsValidType A} {E: EqvType A}, P S -> P (S_Intersect S))
+    (f_vtype: forall {A: Set} {S: Subtype A} {V: IsValidType A} {E: EqvType A}, P S -> P (S_vtype S))
+    (f_otype: forall {A: Set} {S: Subtype A} {V: IsValidType A} {E: EqvType A}, P S -> P (S_otype S))
+    (f_tparam: forall {A: Set} {S: Subtype A} {V: IsValidType A} {E: EqvType A}, P S -> P (S_tparam S))
+    (f_itype: forall {A: Set} {S: Subtype A} {V: IsValidType A} {E: EqvType A}, P S -> P (S_itype S))
+    (f_stype: forall {A: Set} {S: Subtype A} {V: IsValidType A} {E: EqvType A}, P S -> P (S_stype S))
+    (f_variance: P S_variance),
+    (P S_ftype -> P S_ftype) -> P S_ftype.
 
 (* Now we prove that these relations are valid *)
-Global Instance Top_option: Top1 option := fun _ _ => None.
-Global Instance Bottom_option: Bottom1 option := @Some.
-Global Instance IsValidType_option: IsValidType1 option := @Option_Forall.
-Global Instance SubtypeRefl_option: SubtypeRefl1 option.
-Proof. intros A S V C a; destruct a; constructor; apply subtype_refl; inv H; assumption. Qed.
-Global Instance SubtypeAntisym_option: SubtypeAntisym1 option.
-Proof. intros A S E C a b H H0; destruct a, b; inv H H0; constructor; apply subtype_antisym; assumption. Qed.
-Global Instance SubtypeTrans_option: SubtypeTrans1 option.
-Proof. intros A S C a b c H H0; destruct a, b, c; inv H H0; constructor; apply subtype_trans with a0; assumption. Qed.
+Global Instance SubtypeRefl_option {A: Set} `(_SubtypeRefl: SubtypeRefl A): SubtypeRefl (S_option subtype).
+Proof. intros a; destruct a; constructor; apply subtype_refl; inv H; assumption. Qed.
+Global Instance SubtypeAntisym_option {A: Set} `(_SubtypeAntisym: SubtypeAntisym A): SubtypeAntisym (S_option subtype).
+Proof. intros a b H H0; destruct a, b; inv H H0; constructor; apply subtype_antisym; assumption. Qed.
+Global Instance SubtypeTrans_option {A: Set} `{_SubtypeTrans: SubtypeTrans A}: SubtypeTrans (S_option subtype).
+Proof. intros a b c H H0; destruct a, b, c; inv H H0; constructor; apply subtype_trans with a0; assumption. Qed.
 
-Global Instance IsValidType_list: IsValidType1 list := @List.Forall.
-Global Instance SubtypeRefl_Zip: @SubtypeRefl1 list S1Of_Zip IsValidType_list.
-Proof. intros A S V C a; induction a; constructor; [apply subtype_refl | apply IHa]; inv H; assumption. Qed.
-Global Instance SubtypeAntisym_Zip: @SubtypeAntisym1 list S1Of_Zip E1Of_Zip.
-Proof. intros A S E C a b H H0; (induction2 a b using ind_list2); [inv H H0 | inv H0 H1 .. ]; constructor; [apply subtype_antisym | apply H]; assumption. Qed.
-Global Instance SubtypeTrans_Zip: @SubtypeTrans1 list S1Of_Zip.
-Proof. intros A S C a b c H H0; (induction3 a b c using ind_list3); [inv H H0 | inv H0 H1 ..]; constructor; [apply subtype_trans with y | apply H]; assumption. Qed.
+Global Instance SubtypeRefl_Zip {A: Set} `{_SubtypeRefl: SubtypeRefl A}: SubtypeRefl (S_Zip subtype).
+Proof. intros a; induction a; constructor; [apply subtype_refl | apply IHa]; inv H; assumption. Qed.
+Global Instance SubtypeAntisym_Zip {A: Set} `{_SubtypeAntisym: SubtypeAntisym A}: SubtypeAntisym (S_Zip subtype).
+Proof. intros a b H H0; (induction2 a b using ind_list2); [inv H H0 | inv H0 H1 .. ]; constructor; [apply subtype_antisym | apply H]; assumption. Qed.
+Global Instance SubtypeTrans_Zip {A: Set} `{_SubtypeTrans: SubtypeTrans A}: SubtypeTrans (S_Zip subtype).
+Proof. intros a b c H H0; (induction3 a b c using ind_list3); [inv H H0 | inv H0 H1 ..]; constructor; [apply subtype_trans with y | apply H]; assumption. Qed.
 
-Global Instance IsValidType_js_record: IsValidType1 js_record := @JsRecordNoDupForall.
-Global Instance SubtypeRefl_JsrZip: @SubtypeRefl1 js_record S1Of_JsrZip IsValidType_js_record.
-Proof. intros A S V C a; induction a; [constructor; constructor |]; destruct a as [ka va]; intros; apply JsRecord1Rel_cons with va a0; [apply subtype_refl | apply IHa | apply JsRecordAdd_head |]; inv H; assumption. Qed.
-Global Instance SubtypeAntisym_JsrZip: @SubtypeAntisym1 js_record S1Of_JsrZip E1Of_JsrZip.
+Global Instance SubtypeRefl_JsrZip {A: Set} `{_SubtypeRefl: SubtypeRefl A}: SubtypeRefl (S_JsrZip subtype).
+Proof. intros a; induction a; [constructor; constructor |]; destruct a as [ka va]; intros; apply JsRecord1Rel_cons with va a0; [apply subtype_refl | apply IHa | apply JsRecordAdd_head |]; inv H; assumption. Qed.
+Global Instance SubtypeAntisym_JsrZip {A: Set} `{_SubtypeAntisym: SubtypeAntisym A}: SubtypeAntisym (S_JsrZip subtype).
 Proof.
-  intros A S E C a b H H0; pose (JsRecord1Rel_In H); pose (JsRecord1Rel_In H0); apply JsRecordRel_In0; try assumption.
+  intros a b H H0; pose (JsRecord1Rel_In H); pose (JsRecord1Rel_In H0); apply JsRecordRel_In0; try assumption.
   - eapply proj1, JsRecord1Rel_NoDup; exact H.
   - eapply proj1, JsRecord1Rel_NoDup; exact H0.
-  - split; intros; [apply (@JsRecord1Rel_HasKey A S) with a | apply (@JsRecord1Rel_HasKey A S) with b]; assumption.
+  - split; intros; [apply (@JsRecord1Rel_HasKey A S0) with a | apply (@JsRecord1Rel_HasKey A S0) with b]; assumption.
   - intros; apply subtype_antisym; [apply s with k | apply s0 with k]; assumption.
 Qed.
-Global Instance SubtypeTrans_JsrZip: @SubtypeTrans1 js_record S1Of_JsrZip.
+Global Instance SubtypeTrans_JsrZip {A: Set} `{_SubtypeTrans: SubtypeTrans A}: SubtypeTrans (S_JsrZip subtype).
 Proof.
-  intros A S C a b c H H0; pose (JsRecord1Rel_In H); pose (JsRecord1Rel_In H0); apply JsRecord1Rel_In0; try assumption.
+  intros a b c H H0; pose (JsRecord1Rel_In H); pose (JsRecord1Rel_In H0); apply JsRecord1Rel_In0; try assumption.
   - eapply proj1, JsRecord1Rel_NoDup; exact H.
   - eapply proj2, JsRecord1Rel_NoDup; exact H0.
-  - intros; apply (@JsRecord1Rel_HasKey A S) with b, (@JsRecord1Rel_HasKey A S) with c; assumption.
-  - intros; destruct (JsRecordHasKey_dec k b); [| contradict H3; apply (@JsRecord1Rel_HasKey A S) with c; [| apply JsRecordHasKey_In0 with vy]; assumption]; rewrite JsRecordHasKey_In in H3; destruct H3 as [vb H3].
+  - intros; apply (@JsRecord1Rel_HasKey A S0) with b, (@JsRecord1Rel_HasKey A S0) with c; assumption.
+  - intros; destruct (JsRecordHasKey_dec k b); [| contradict H3; apply (@JsRecord1Rel_HasKey A S0) with c; [| apply JsRecordHasKey_In0 with vy]; assumption]; rewrite JsRecordHasKey_In in H3; destruct H3 as [vb H3].
     apply subtype_trans with vb; [apply s with k | apply s0 with k]; assumption.
 Qed.
 
@@ -323,87 +294,80 @@ Lemma S_Intersect_length_antisym {A: Set} {S: Subtype A}: forall (xs ys: list A)
 Proof. intros; apply Nat.le_antisymm; apply S_Intersect_length; assumption. Qed.
 Local Ltac discr_on_intersect_length := lazymatch goal with | H: [S_Intersect _] _ <: _, H0: [S_Intersect _] _ <: _ |- _ => let e := fresh "e" in let e0 := fresh "e0" in pose' (S_Intersect_length H) as e; pose' (S_Intersect_length H0) as e0; simpl in e, e0 end; lia.
 
-Global Instance SubtypeRefl_Intersect: @SubtypeRefl1 list S1Of_Intersect IsValidType_list.
-Proof. intros A S V C a; induction a; constructor; [apply subtype_refl | apply IHa]; inv H; assumption. Qed.
-Global Instance SubtypeAntisym_Intersect: @SubtypeAntisym1 list S1Of_Intersect E1Of_Zip.
+Global Instance SubtypeRefl_Intersect {A: Set} `{_SubtypeRefl: SubtypeRefl A}: SubtypeRefl (S_Intersect subtype).
+Proof. intros a; induction a; constructor; [apply subtype_refl | apply IHa]; inv H; assumption. Qed.
+Global Instance SubtypeAntisym_Intersect {A: Set} `{_SubtypeAntisym: SubtypeAntisym A}: SubtypeAntisym (S_Intersect subtype).
 Proof.
-  intros A S E C a b H H0; pose' (S_Intersect_length_antisym H H0); (induction2 a b using ind_list2); simpl in e;
+  intros a b H H0; pose' (S_Intersect_length_antisym H H0); (induction2 a b using ind_list2); simpl in e;
     [constructor | discriminate e | discriminate e |]; inv e H0 H1; try discr_on_intersect_length;
     constructor; [apply subtype_antisym | apply H]; assumption.
 Qed.
-Global Instance SubtypeTrans_Intersect: @SubtypeTrans1 list S1Of_Intersect.
+Global Instance SubtypeTrans_Intersect {A: Set} `{_SubtypeTrans: SubtypeTrans A}: SubtypeTrans (S_Intersect subtype).
 Proof.
-  intros A S C a; induction a; try rename a into a0, a0 into a; induction b; try rename a1 into b0; induction c; try rename a1 into c0; intros;
+  intros a; induction a; try rename a into a0, a0 into a; induction b; try rename a1 into b0; induction c; try rename a1 into c0; intros;
     try (inv H H0; fail); [constructor .. |]; inv H H0;
     [constructor; [apply subtype_trans with b0 | apply IHa with b] | apply IHb; [constructor |] | constructor; apply IHa with (b0 :: b); [| constructor] ..]; assumption.
 Qed.
 
-Global Instance Top_variance: Top variance := Bivariant.
-Global Instance Bottom_variance: Bottom variance := Invariant.
-Global Instance IsValidType_variance: IsValidType variance := IsValidType_always.
-Global Instance SubtypeRefl_variance: SubtypeRefl variance.
+Global Instance SubtypeRefl_variance: SubtypeRefl S_variance.
 Proof. intros a; destruct a; constructor. Qed.
-Global Instance SubtypeAntisym_variance: SubtypeAntisym variance.
+Global Instance SubtypeAntisym_variance: SubtypeAntisym S_variance.
 Proof. intros a b H H0; destruct a, b; inv H H0; constructor. Qed.
-Global Instance SubtypeTrans_variance: SubtypeTrans variance.
+Global Instance SubtypeTrans_variance: SubtypeTrans S_variance.
 Proof. intros a b c H H0; destruct a, b, c; inv H H0; constructor. Qed.
 
-Global Instance Top_otype: Top1 otype := fun _ top => Ot true top.
-Global Instance Bottom_otype: Bottom1 otype := fun _ bottom => Ot false bottom.
-Global Instance IsValidType_otype: IsValidType1 otype := @OType_Forall.
-Global Instance SubtypeRefl_otype: SubtypeRefl1 otype.
-Proof. intros A S V C a; destruct a; constructor; [destruct optional; simpl; reflexivity | apply subtype_refl]; inv H; assumption. Qed.
-Global Instance SubtypeAntisym_otype: SubtypeAntisym1 otype.
-Proof. intros A S E C a b H H0; destruct a, b; inv H H0; destruct optional, optional0; try discriminate; constructor; apply subtype_antisym; assumption. Qed.
-Global Instance SubtypeTrans_otype: SubtypeTrans1 otype.
-Proof. intros A S C a b c H H0; destruct a, b, c; inv H H0; destruct optional, optional0, optional1; try discriminate; constructor; (simpl; reflexivity) || apply subtype_trans with a0; assumption. Qed.
+Global Instance SubtypeRefl_otype {A: Set} `{_SubtypeRefl: SubtypeRefl A}: SubtypeRefl (S_otype subtype).
+Proof. intros a; destruct a; constructor; [destruct optional; simpl; reflexivity | apply subtype_refl]; inv H; assumption. Qed.
+Global Instance SubtypeAntisym_otype {A: Set} `{_SubtypeAntisym: SubtypeAntisym A}: SubtypeAntisym (S_otype subtype).
+Proof. intros a b H H0; destruct a, b; inv H H0; destruct optional, optional0; try discriminate; constructor; apply subtype_antisym; assumption. Qed.
+Global Instance SubtypeTrans_otype {A: Set} `{_SubtypeTrans: SubtypeTrans A}: SubtypeTrans (S_otype subtype).
+Proof. intros a b c H H0; destruct a, b, c; inv H H0; destruct optional, optional0, optional1; try discriminate; constructor; (simpl; reflexivity) || apply subtype_trans with a0; assumption. Qed.
 
-Global Instance IsValidType_vtype: IsValidType1 vtype := @VType_Forall.
-Global Instance SubtypeRefl_vtype: SubtypeRefl1 vtype.
-Proof. intros A S V C a; destruct a; constructor; apply subtype_refl; inv H; assumption. Qed.
-Global Instance SubtypeAntisym_vtype: SubtypeAntisym1 vtype.
-Proof. intros A S E C a b H H0; destruct a, b; inv H H0; constructor; apply subtype_antisym; assumption. Qed.
-Global Instance SubtypeTrans_vtype: SubtypeTrans1 vtype.
-Proof. intros A S C a b c H H0; destruct a, b, c; inv H H0; constructor; apply subtype_trans with a0; assumption. Qed.
+Global Instance SubtypeRefl_vtype {A: Set} `{_SubtypeRefl: SubtypeRefl A}: SubtypeRefl (S_vtype subtype).
+Proof. intros a; destruct a; constructor; apply subtype_refl; inv H; assumption. Qed.
+Global Instance SubtypeAntisym_vtype {A: Set} `{_SubtypeAntisym: SubtypeAntisym A}: SubtypeAntisym (S_vtype subtype).
+Proof. intros a b H H0; destruct a, b; inv H H0; constructor; apply subtype_antisym; assumption. Qed.
+Global Instance SubtypeTrans_vtype {A: Set} `{_SubtypeTrans: SubtypeTrans A}: SubtypeTrans (S_vtype subtype).
+Proof. intros a b c H H0; destruct a, b, c; inv H H0; constructor; apply subtype_trans with a0; assumption. Qed.
 
-Global Instance IsValidType_tparam: IsValidType1 tparam := @TParam_Forall.
-Global Instance SubtypeRefl_tparam: SubtypeRefl1 tparam.
-Proof. intros A S V C a; destruct a; constructor; [apply subtype_refl | apply (SubtypeRefl_Intersect subtype_refl)]; [reflexivity | inv H; assumption]. Qed.
-Global Instance SubtypeAntisym_tparam: SubtypeAntisym1 tparam.
-Proof. intros A S E C a b H H0; destruct a, b; inv H H0; rewrite (SubtypeAntisym_variance H2 H3); constructor; apply (SubtypeAntisym_Intersect subtype_antisym); assumption. Qed.
-Global Instance SubtypeTrans_tparam: SubtypeTrans1 tparam.
-Proof. intros A S C a b c H H0; destruct a, b, c; inv H H0; constructor; [apply subtype_trans with v0 | apply (SubtypeTrans_Intersect subtype_trans) with supers0]; assumption. Qed.
+Global Instance SubtypeRefl_tparam {A: Set} `{_SubtypeRefl: SubtypeRefl A}: SubtypeRefl (S_tparam subtype).
+Proof. intros a; destruct a; constructor; apply subtype_refl; [reflexivity | inv H; assumption]. Qed.
+Global Instance SubtypeAntisym_tparam {A: Set} `{_SubtypeAntisym: SubtypeAntisym A}: SubtypeAntisym (S_tparam subtype).
+Proof. intros a b H H0; destruct a, b; inv H H0; rewrite (SubtypeAntisym_variance H2 H3); constructor; apply SubtypeAntisym_Intersect; assumption. Qed.
+Global Instance SubtypeTrans_tparam {A: Set} `{_SubtypeTrans: SubtypeTrans A}: SubtypeTrans (S_tparam subtype).
+Proof. intros a b c H H0; destruct a, b, c; inv H H0; constructor; [apply subtype_trans with v0 | apply subtype_trans with supers0]; assumption. Qed.
 
-Global Instance IsValidType_itype: IsValidType1 itype := @IType_Forall.
-Global Instance SubtypeRefl_itype: SubtypeRefl1 itype.
-Proof. intros A S V C a; destruct a; constructor; apply (SubtypeRefl_Zip subtype_refl); inv H; assumption. Qed.
-Global Instance SubtypeAntisym_itype: SubtypeAntisym1 itype.
-Proof. intros A S E C a b H H0; destruct a, b; inv H H0; constructor; apply (SubtypeAntisym_Zip subtype_antisym); assumption. Qed.
-Global Instance SubtypeTrans_itype: SubtypeTrans1 itype.
-Proof. intros A S C a b c H H0; destruct a, b, c; inv H H0; constructor; apply (SubtypeTrans_Zip subtype_trans) with targs0; assumption. Qed.
+Global Instance SubtypeRefl_itype {A: Set} `{_SubtypeRefl: SubtypeRefl A}: SubtypeRefl (S_itype subtype).
+Proof. intros a; destruct a; constructor; apply subtype_refl; inv H; assumption. Qed.
+Global Instance SubtypeAntisym_itype {A: Set} `{_SubtypeAntisym: SubtypeAntisym A}: SubtypeAntisym (S_itype subtype).
+Proof. intros a b H H0; destruct a, b; inv H H0; constructor; apply SubtypeAntisym_Zip; assumption. Qed.
+Global Instance SubtypeTrans_itype {A: Set} `{_SubtypeTrans: SubtypeTrans A}: SubtypeTrans (S_itype subtype).
+Proof. intros a b c H H0; destruct a, b, c; inv H H0; constructor; apply subtype_trans with targs0; assumption. Qed.
 
-Global Instance IsValidType_stype: IsValidType1 stype := @SType_Forall'.
-Global Instance SubtypeRefl_stype: SubtypeRefl1 stype.
-Proof. intros A S V C a; destruct a; constructor; (apply subtype_refl || apply (SubtypeRefl_Zip (SubtypeRefl_tparam subtype_refl)) || apply (SubtypeRefl_Zip (SubtypeRefl_otype subtype_refl)) || apply (SubtypeRefl_JsrZip (SubtypeRefl_otype subtype_refl)) || apply (SubtypeRefl_vtype subtype_refl)); inv H; assumption || (eapply unIsValidType1'; eassumption). Qed.
-Global Instance SubtypeAntisym_stype: SubtypeAntisym1 stype.
-Proof. intros A S E C a b H H0; destruct a, b; inv H H0; constructor; (apply subtype_antisym || apply (SubtypeAntisym_Zip (SubtypeAntisym_tparam subtype_antisym)) || apply (SubtypeAntisym_Zip (SubtypeAntisym_otype subtype_antisym)) || apply (SubtypeAntisym_JsrZip (SubtypeAntisym_otype subtype_antisym)) || apply (SubtypeAntisym_vtype subtype_antisym)); assumption. Qed.
-Global Instance SubtypeTrans_stype: SubtypeTrans1 stype.
-Proof. intros A S C a b c H H0; destruct a, b, c; inv H H0; constructor; (eapply subtype_trans || eapply (SubtypeTrans_Zip (SubtypeTrans_tparam subtype_trans)) || eapply (SubtypeTrans_Zip (SubtypeTrans_otype subtype_trans)) || eapply (SubtypeTrans_JsrZip (SubtypeTrans_otype subtype_trans)) || eapply (SubtypeTrans_vtype subtype_trans)); eassumption.
-Unshelve. exact (SubtypeTrans_Zip (SubtypeTrans_tparam subtype_trans)). exact (SubtypeTrans_Zip (SubtypeTrans_otype subtype_trans)). exact (SubtypeTrans_vtype subtype_trans). exact (SubtypeTrans_Zip (SubtypeTrans_otype subtype_trans)). exact (SubtypeTrans_JsrZip (SubtypeTrans_otype subtype_trans)). Qed.
+Global Instance SubtypeRefl_stype: forall {A: Set} `{_SubtypeRefl: SubtypeRefl A}, SubtypeRefl (S_stype subtype).
+Proof. intros A S0 V S a; destruct a; constructor; apply subtype_refl; inv H; assumption. Qed.
+Global Instance SubtypeAntisym_stype {A: Set} `{_SubtypeAntisym: SubtypeAntisym A}: SubtypeAntisym (S_stype subtype).
+Proof. intros a b H H0; destruct a, b; inv H H0; constructor; apply subtype_antisym || apply SubtypeAntisym_Zip; assumption. Qed.
+Global Instance SubtypeTrans_stype {A: Set} `{_SubtypeTrans: SubtypeTrans A}: SubtypeTrans (S_stype subtype).
+Proof. intros a b c H H0; destruct a, b, c; inv H H0; constructor; eapply subtype_trans; eassumption. Qed.
 
-Inductive _IsValidType_ftype: ftype -> Prop :=
-| FAny: _IsValidType_ftype FAny
-| FNever: forall x, _IsValidType_ftype (FNever x)
-| FStructural: forall x structure, @IsValidType_stype ftype _IsValidType_ftype structure -> _IsValidType_ftype (FStructural x structure)
-| FNominal: forall x id sids structure, @IsValidType_itype ftype _IsValidType_ftype id -> @IsValidType_list iftype (@IsValidType_itype ftype _IsValidType_ftype) sids -> @IsValidType_option sftype (@IsValidType_stype ftype _IsValidType_ftype) structure -> _IsValidType_ftype (FNominal x id sids structure)
-.
-Global Instance IsValidType_ftype: IsValidType ftype := _IsValidType_ftype.
-Fixpoint SubtypeRefl_ftype (a: ftype) (V: is_valid_type a): a <: a.
-destruct a.
+Local Ltac rewrite_lia a b := let H := fresh "H" in assert (H: a = b); [lia |]; rewrite H; clear H.
+Global Instance SubtypeRefl_ftype: SubtypeRefl S_ftype.
+intros a; remember (ftype_depth a) as n; assert (Hle : (ftype_depth a <= n)%nat); [lia |]; clear Heqn; revert Hle; revert a; induction n; intros; [destruct a; simpl in Hle; lia | destruct a; simpl in Hle; inv H].
 - constructor.
 - destruct nullable; constructor; reflexivity.
-- constructor; inv V; [destruct nullable; reflexivity |]; apply subtype_refl1; assumption.
-- constructor; inv V; [destruct nullable; reflexivity | ..]; eapply subtype_refl1.
+- constructor; [destruct nullable; reflexivity |]. unshelve eapply subtype_refl; [| | exact H1]; unfold SubtypeRefl.
+- constructor; [destruct nullable; reflexivity |].
+apply S_ftype_ind0; intros.
+intros a V; induction a using ftype_ind'.
+- constructor.
+- destruct nullable; constructor; reflexivity.
+- constructor; inv V; [destruct nullable; reflexivity |]; eapply subtype_refl; eassumption.
+- constructor; inv V; [destruct nullable; reflexivity | ..]; eapply subtype_refl; [apply List.Forall_cons |]; eassumption.
+Unshelve. eapply SubtypeRefl_stype. eapply SubtypeRefl_Intersect. eapply SubtypeRefl_option; eapply SubtypeRefl_stype.
+Unshelve. unfold SubtypeRefl; auto. unfold SubtypeRefl; auto. eapply SubtypeRefl_itype. unfold SubtypeRefl; auto.
+Unshelve. unfold SubtypeRefl; auto. Defined.
+Defined.
 Global Instance SubtypeRefl_ftype {A: Set}: SubtypeRefl ftype.
 Ltac inv_con :=
   lazymatch goal with
